made the first step to support physical subtyping: the momery load checks if data in memory match the low level type information given by load, returns undef if not; memory data take low level type information from memory store; the low-level type information include int with arbitrary precision, float, pointers from malloc, pointers casted from int; pointers are always of 32-bit.
Also fixed all admitted lemmas in our memory model.
One external tool is required for psatz tactics (solving Z arithmetic):
  https://projects.coin-or.org/Csdp
Adding its bin path into PATH should work.



git-svn-id: https://webdav.seas.upenn.edu/svn/sol/vol@2973 eef5ea85-cc2e-0410-bd84-0fae1f012da8

src/ssa/compcert/Memdata.v
@@ -117,7 +117,7 @@ Definition align_chunk (chunk: memory_chunk) : Z :=
   | Mint wz => 
     if le_lt_dec wz 31
     then bytesize_chunk wz
-    else 4
+    else if zeq (bytesize_chunk wz) 8 then 4 else 1
   | _ => 4
   end.
 
@@ -127,55 +127,86 @@ Proof.
   intro. destruct chunk; simpl; try omega.
     destruct (le_lt_dec n 31); try omega.
       apply bytesize_chunk_pos.
+      destruct (zeq (bytesize_chunk n) 8); omega.
 Qed.
 
-(*
+Lemma bytesize_chunk_7_eq_1 : bytesize_chunk 7 = 1.
+Proof. compute. auto. Qed.
+
+Lemma bytesize_chunk_31_eq_4 : bytesize_chunk 31 = 4.
+Proof. compute. auto. Qed.
+
+Lemma bytesize_chunk_63_eq_8 : bytesize_chunk 63 = 8.
+Proof. compute. auto. Qed.
+
 Lemma align_size_chunk_divides:
   forall chunk, (align_chunk chunk | size_chunk chunk).
 Proof.
   intros. destruct chunk; simpl; try solve [
     apply Zdivide_refl |
-    destruct (le_lt_dec n 3); auto with zarith |
+    destruct (le_lt_dec n 31); auto with zarith |
     exists 2; auto ]. 
 
-    destruct (le_lt_dec n 3); auto with zarith.
+    destruct (le_lt_dec n 31); auto with zarith.
+    destruct (zeq (bytesize_chunk n) 8); auto with zarith.
+      rewrite e.
+      assert (8 = 2 * 4) as EQ. auto with zarith.
+      rewrite EQ.
+      apply Zdivide_factor_l.
 Qed.
-*)
 
-Lemma bytesize_chunk_7_eq_1 : bytesize_chunk 7 = 1.
+Lemma bytesize_chunk_le : forall n m,
+  (m <= n)%nat ->
+  bytesize_chunk m <= bytesize_chunk n.  
 Proof.
-  unfold bytesize_chunk.
-  unfold ZRdiv. compute. auto.
-Qed.
+  intros n m H.
+  unfold bytesize_chunk, ZRdiv.
+  simpl.
+  assert (Zpos (P_of_succ_nat m) <= Zpos (P_of_succ_nat n)) as A.
+    apply Zpos_P_of_succ_nat_mono; auto.
 
-Lemma bytesize_chunk_31_eq_4 : bytesize_chunk 31 = 4.
-Proof.
-  unfold bytesize_chunk.
-  unfold ZRdiv. compute. auto.
+  remember (Zpos (P_of_succ_nat m)) as z1.
+  remember (Zpos (P_of_succ_nat n)) as z2.
+  assert (z1 > 0) as C. rewrite Heqz1. auto with zarith.
+  clear - A C.
+  assert (z1 / 8 <= z2 / 8) as B.
+    apply Z_div_le; auto with zarith.
+  destruct (zeq (z1 mod 8) 0).
+    destruct (zeq (z2 mod 8) 0); auto with zarith.
+    destruct (zeq (z2 mod 8) 0); auto with zarith.
+      assert (z1 = 8*(z1/8) + (z1 mod 8)) as Z1.
+        apply Z_div_mod_eq; auto with zarith.
+      assert (z2 = 8*(z2/8) + (z2 mod 8)) as Z2.
+        apply Z_div_mod_eq; auto with zarith.
+      rewrite e in Z2.
+      assert (0 <= z1 mod 8 < 8) as D.
+        apply Z_mod_lt; auto with zarith.
+      destruct (Z_le_dec (z1 / 8 + 1) (z2 / 8)); auto.
+        contradict A.
+        rewrite Z1. rewrite Z2.
+        clear Z1 Z2 e. auto with zarith.
 Qed.
-
-Lemma bytesize_chunk_63_eq_8 : bytesize_chunk 63 = 8.
-Proof.
-  unfold bytesize_chunk.
-  unfold ZRdiv. compute. auto.
-Qed.
-
+ 
 Lemma bytesize_chunk_le_31 : forall n,
-  (n <= 31)%nat ->
-  bytesize_chunk n <= 4.
+  (n <= 31)%nat -> bytesize_chunk n <= 4.
 Proof.
-  unfold bytesize_chunk.
-  unfold ZRdiv.
-  intros.
-  destruct n.
-    compute. intro. inversion H0.
-Admitted.
+  intros. 
+  rewrite <- bytesize_chunk_31_eq_4.
+  apply bytesize_chunk_le; auto.
+Qed.
+
+Lemma bytesize_chunk_32_eq_5 : bytesize_chunk 32 = 5.
+Proof. compute. auto. Qed.
 
 Lemma bytesize_chunk_gt_31 : forall n,
-  (31 < n)%nat ->
-  bytesize_chunk n > 4.
+  (31 < n)%nat -> bytesize_chunk n > 4.
 Proof.
-Admitted.
+  intros. 
+  assert ((32 <= n)%nat) as J. auto with zarith.
+  apply bytesize_chunk_le in J.
+  rewrite bytesize_chunk_32_eq_5 in J.
+  auto with zarith.
+Qed.
 
 Lemma bytesize_chunk_31_neq : forall n1 n2,
   (n1 <= 31 < n2)%nat ->
@@ -199,9 +230,20 @@ Proof.
   omega.
 Qed.
 
+Lemma bytesize_chunk_neq : forall n1 n2,
+  (n1 <= 31)%nat -> (n2 > 31)%nat ->
+  bytesize_chunk n1 <> bytesize_chunk n2.
+Proof.
+  intros.
+  apply bytesize_chunk_le_31 in H.
+  apply bytesize_chunk_gt_31 in H0.
+  omega.
+Qed.
+
 Lemma align_chunk_compat:
   forall chunk1 chunk2,
-  size_chunk chunk1 = size_chunk chunk2 -> align_chunk chunk1 = align_chunk chunk2.
+  size_chunk chunk1 = size_chunk chunk2 -> 
+  align_chunk chunk1 = align_chunk chunk2.
 Proof.
   intros chunk1 chunk2. 
   destruct chunk1; destruct chunk2; simpl; try congruence; auto.
@@ -211,17 +253,34 @@ Proof.
       destruct (le_lt_dec n0 31); auto.
         intro. contradict H; auto using bytesize_chunk_31_neq'.
 
-    destruct (le_lt_dec n 31); auto.
+    intro J.
+    destruct (zeq (bytesize_chunk n) 8); auto.
+      destruct (zeq (bytesize_chunk n0) 8); auto.
+        rewrite e in J. rewrite J in n1. contradict n1; auto.
+      destruct (zeq (bytesize_chunk n0) 8); auto.
+        rewrite e in J. rewrite J in n1. contradict n1; auto.
 
+    destruct (le_lt_dec n 31); auto.
+      apply bytesize_chunk_gt_31 in l.
+      intro. rewrite H in l. contradict l; omega.
+
+    intro J. rewrite J.
+    destruct (zeq 8 8) as [ | n']; try solve [contradict n'; auto].
     destruct (le_lt_dec n 31); auto.
       apply bytesize_chunk_le_31 in l.
-      intro. rewrite H in l. contradict l; auto.
+      rewrite J in l. contradict l. omega.
 
+    intro J. rewrite <- J.
+    destruct (zeq 4 8) as [e' | ]; try solve [inversion e'].
     destruct (le_lt_dec n 31); auto.
+      apply bytesize_chunk_gt_31 in l.
+      rewrite J in l. contradict l. omega.
 
+    intro J. rewrite <- J.
+    destruct (zeq 8 8) as [ | n']; try solve [contradict n'; auto].
     destruct (le_lt_dec n 31); auto.
       apply bytesize_chunk_le_31 in l.
-      intro. rewrite <- H in l. contradict l; auto.
+      rewrite <- J in l. contradict l. omega.
 Qed.
 
 Definition chunk_eq (c1 c2:memory_chunk) : Prop :=
@@ -258,18 +317,57 @@ Inductive memval: Type :=
 (** We define functions to convert between integers and lists of bytes
   according to a given memory chunk. *)
 
-(** bytes_of_int *)
-
 Fixpoint bytes_of_int (n: nat) (x: Z) {struct n}: list byte :=
   match n with
   | O => nil
   | S m => Int.repr 7 x :: bytes_of_int m (x / 256)
   end.
 
+Fixpoint int_of_bytes (l: list byte): Z :=
+  match l with
+  | nil => 0
+  | b :: l' => Int.unsigned 7 b + int_of_bytes l' * 256
+  end.
+
 Lemma length_bytes_of_int:
   forall n x, length (bytes_of_int n x) = n.
 Proof.
   induction n; simpl; intros. auto. decEq. auto.
+Qed.
+
+
+Lemma int_of_bytes_of_int:
+  forall n x,
+  int_of_bytes (bytes_of_int n x) = x mod (two_p (Z_of_nat n * 8)).
+Proof.
+  induction n; intros.
+  simpl. rewrite Zmod_1_r. auto.
+  rewrite inj_S. simpl.
+  replace (Zsucc (Z_of_nat n) * 8) with (Z_of_nat n * 8 + 8) by omega.
+  rewrite two_p_is_exp; try omega. 
+  rewrite Zmod_recombine. rewrite IHn. rewrite Zplus_comm. reflexivity. 
+  apply two_p_gt_ZERO. omega. apply two_p_gt_ZERO. omega.
+Qed.
+
+Lemma int_of_bytes_of_int_wz:
+  forall n wz x,
+  0 < Z_of_nat n ->
+  Int.repr wz (int_of_bytes (bytes_of_int n (Int.unsigned wz x))) = 
+  Int.zero_ext wz (Z_of_nat n * 8) x.
+Proof.
+  intros. rewrite int_of_bytes_of_int. 
+  rewrite <- (Int.repr_unsigned wz (Int.zero_ext wz (Z_of_nat n * 8) x)). 
+  decEq. symmetry. apply Int.zero_ext_mod; try solve [omega]. 
+Qed.
+
+Lemma int_of_bytes_of_int_2:
+  forall n x,
+  (n = 1 \/ n = 2)%nat ->
+  Int.repr 31 (int_of_bytes (bytes_of_int n (Int.unsigned 31 x))) = 
+    Int.zero_ext 31 (Z_of_nat n * 8) x.
+Proof.
+  intros. apply int_of_bytes_of_int_wz.
+  destruct H; subst n; compute; auto.
 Qed.
 
 Lemma bytes_of_int_mod:
@@ -318,235 +416,6 @@ Proof.
     auto.
 Qed.
 
-(** int_of_bytes *)
-
-Fixpoint int_of_bytes (l: list byte): Z :=
-  match l with
-  | nil => 0
-  | b :: l' => Int.unsigned 7 b + int_of_bytes l' * 256
-  end.
-
-Lemma int_of_bytes_of_int:
-  forall n x,
-  int_of_bytes (bytes_of_int n x) = x mod (two_p (Z_of_nat n * 8)).
-Proof.
-  induction n; intros.
-  simpl. rewrite Zmod_1_r. auto.
-  rewrite inj_S. simpl.
-  replace (Zsucc (Z_of_nat n) * 8) with (Z_of_nat n * 8 + 8) by omega.
-  rewrite two_p_is_exp; try omega. 
-  rewrite Zmod_recombine. rewrite IHn. rewrite Zplus_comm. reflexivity. 
-  apply two_p_gt_ZERO. omega. apply two_p_gt_ZERO. omega.
-Qed.
-
-Lemma int_of_bytes_of_int_wz:
-  forall n wz x,
-  0 < Z_of_nat n ->
-  Int.repr wz (int_of_bytes (bytes_of_int n (Int.unsigned wz x))) = 
-  Int.zero_ext wz (Z_of_nat n * 8) x.
-Proof.
-  intros. rewrite int_of_bytes_of_int. 
-  rewrite <- (Int.repr_unsigned wz (Int.zero_ext wz (Z_of_nat n * 8) x)). 
-  decEq. symmetry. apply Int.zero_ext_mod; try solve [omega]. 
-Qed.
-
-Lemma int_of_bytes_of_int_2:
-  forall n x,
-  (n = 1 \/ n = 2)%nat ->
-  Int.repr 31 (int_of_bytes (bytes_of_int n (Int.unsigned 31 x))) = Int.zero_ext 31 (Z_of_nat n * 8) x.
-Proof.
-  intros. apply int_of_bytes_of_int_wz.
-  destruct H; subst n; compute; auto.
-Qed.
-
-Definition inj_bytes (bl: list byte) : list memval :=
-  List.map (Byte 8) bl.
-
-Remark length_inj_bytes:
-  forall bl, length (inj_bytes bl) = length bl.
-Proof.
-  intros. apply List.map_length. 
-Qed.
-
-(** inj_int *)
-
-Definition inj_int (wz:nat) (x: Int.int wz) : list memval :=
-  let z := Int.unsigned wz x in
-  let n := Z_of_nat (S wz) in
-  let m := n mod 8 in
-  let sz := ZRdiv n 8 in
-  let bl := bytes_of_int (nat_of_Z sz) z in
-  match bl with
-  | nil => nil
-  | b::bl' => Byte (nat_of_Z m) b :: inj_bytes bl'
-  end.
-
-Lemma length_inj_int : forall wz n,
-  length (inj_int wz n) = bytesize_chunk_nat wz.
-Proof.
-  intros.
-  unfold inj_int, bytesize_chunk_nat, bytesize_chunk.
-  assert (J:=@length_bytes_of_int 
-    (nat_of_Z (ZRdiv (Z_of_nat (S wz)) 8)) 
-    (Int.unsigned wz n)).
-  remember (bytes_of_int (nat_of_Z (ZRdiv (Z_of_nat (S wz)) 8)) 
-    (Int.unsigned wz n)) as bl.
-  destruct bl; auto.
-    simpl in *.
-    rewrite <- J.
-    decEq.
-    apply map_length.
-Qed.   
-
-(** proj_bytes *)
-
-Fixpoint proj_bytes (n:nat) (vl: list memval) {struct n} : option (list byte) :=
-  match n, vl with
-  | O, nil => Some nil
-  | S m, Byte wz b :: vl' =>
-      if eq_nat_dec wz 8 
-      then
-        match (proj_bytes m vl') with
-        | Some bl' => Some (b :: bl')
-        | None => None
-        end
-      else None
-  | _, _ => None
-  end.
-
-Remark proj_inj_bytes:
-  forall bl, proj_bytes (length bl) (inj_bytes bl) = Some bl.
-Proof.
-  induction bl; simpl. auto. rewrite IHbl. auto.
-Qed.
-
-Lemma inj_proj_bytes:
-  forall cl bl, proj_bytes (length cl) cl = Some bl -> cl = inj_bytes bl.
-Proof.
-  induction cl; simpl; intros. 
-  inv H; auto.
-  destruct a; try congruence.
-  destruct (eq_nat_dec n 8); subst.
-    destruct (proj_bytes (length cl) cl); inv H.
-      simpl. decEq. auto.
-      inversion H.
-Qed.
-
-Lemma proj_bytes_prop1 : forall n wz x bl,
-  proj_bytes n (map (Byte 8) (bytes_of_int n (Int.unsigned wz x / 256))) = Some bl ->
-  x = Int.repr wz (Int.unsigned wz x mod Int.modulus 7 + int_of_bytes bl * 256).
-Proof.
-  intros.
-  
-Admitted.
-
-Lemma proj_bytes_prop2: forall vl n,
-  length vl = n ->
-  exists bl, proj_bytes n (map (Byte 8) vl) = Some bl.
-Proof.
-  induction vl; intros; subst; simpl.
-    exists nil. auto.
-    
-    destruct (@IHvl (length vl)) as [bl J]; auto.
-    rewrite J.
-    exists (a::bl). auto.
-Qed.
-
-Lemma proj_bytes_prop3: forall vl n bl,
-  proj_bytes n (map (Byte 8) vl) = Some bl ->
-  length bl = n /\ length vl = n.
-Admitted.
-
-(** proj_int *)
-
-Definition proj_int (wz:nat) (vl: list memval) : option (Int.int wz) :=
-  let n := Z_of_nat (S wz) in
-  let m := nat_of_Z (n mod 8) in
-  let sz := nat_of_Z (ZRdiv n 8) in
-  match sz, vl with
-  | O, nil => None
-  | S n', Byte wz0 b :: vl' =>
-    if eq_nat_dec wz0 m
-    then 
-      match (proj_bytes n' vl') with
-      | Some bl' => Some (Int.repr wz (int_of_bytes (b::bl')))
-      | None => None
-      end
-    else None
-  | _, _ => None
-  end.
-
-Lemma proj_inj_int_eq : 
-  forall wz x,
-  proj_int wz (inj_int wz x) = Some x.
-Proof.
-  intros.
-  unfold proj_int, inj_int.
-  remember (nat_of_Z (ZRdiv (Z_of_nat (S wz)) 8)) as n.
-  assert (n > 0)%nat.
-    subst.
-    apply ZRdiv_prop6.
-  Opaque Z_of_nat.
-  destruct n; simpl.
-    contradict H; omega.
-
-    destruct (eq_nat_dec 
-      (nat_of_Z ((Z_of_nat (S wz)) mod 8))
-      (nat_of_Z ((Z_of_nat (S wz)) mod 8))
-      ).
-      destruct (@proj_bytes_prop2 (bytes_of_int n (Int.unsigned wz x/256)) n) 
-        as [bl EQ].
-        apply length_bytes_of_int.
-        unfold inj_bytes.
-        rewrite EQ. 
-
-        apply proj_bytes_prop1 in EQ. rewrite <- EQ. auto.
-      contradict n0; auto.
-Qed.
-
-Lemma proj_inj_int_neq : 
-  forall wz1 wz2 x,
-  wz1 <> wz2 ->
-  proj_int wz1 (inj_int wz2 x) = None.
-Proof.
-  intros.
-  unfold proj_int, inj_int.
-  remember (nat_of_Z (ZRdiv (Z_of_nat (S wz1)) 8)) as n.
-  assert (n > 0)%nat.
-    subst.
-    apply ZRdiv_prop6.
-  Opaque Z_of_nat.
-  destruct n; simpl.
-    contradict H; omega.
-    destruct (@bytes_of_int_prop1 
-      (nat_of_Z (ZRdiv (Z_of_nat (S wz2)) 8))
-      (Int.unsigned wz2 x))
-      as [b [bl EQ]].
-      apply ZRdiv_prop6.
-    rewrite EQ.      
-
-    unfold inj_bytes.
-    destruct (eq_nat_dec 
-      (nat_of_Z ((Z_of_nat (S wz2)) mod 8))
-      (nat_of_Z ((Z_of_nat (S wz1)) mod 8))
-      ); auto.
-      apply nat_of_Z_inj in e; try solve [apply mod_prop1].
-        remember (proj_bytes n (map (Byte 8) bl)) as R.
-        destruct R; auto.
-          symmetry in HeqR.
-          apply proj_bytes_prop3 in HeqR.
-          destruct HeqR as [EQ1 EQ2]; subst.
-          assert(J:=@length_bytes_of_int (nat_of_Z (ZRdiv (Z_of_nat (S wz2)) 8)) (Int.unsigned wz2 x)).
-          rewrite EQ in J.
-          simpl in J. rewrite EQ2 in J.
-          rewrite Heqn in J.
-          apply nat_of_Z_inj in J; try solve [apply ZRdiv_prop4].
-            apply zrdiv_zmod_prop1 in J; auto with zarith.
-              apply inj_eq_rev in J; auto.
-              inversion J; subst.        
-              contradict H; auto.
-Qed.
-
 Parameter big_endian: bool.
 
 Definition rev_if_be (A:Type) (l: list A) : list A :=
@@ -568,56 +437,82 @@ Proof.
   auto.
 Qed.
 
-(* generate the stored bytes of x (with size wz). *)
-Definition encode_int (wz:nat) (x: Int.int wz) : list memval :=
-  rev_if_be _ (inj_int wz x).
+Definition encode_int (c:memory_chunk) (wz:nat) (x: Int.int wz) : list byte :=
+  let n := Int.unsigned wz x in
+  rev_if_be _ (match c with
+  | Mint wz0 => bytes_of_int (nat_of_Z (bytesize_chunk wz0)) n
+  | Mfloat32 => bytes_of_int 4%nat 0
+  | Mfloat64 => bytes_of_int 8%nat 0
+  end).
 
-Definition decode_int (b: list memval) (wz:nat) : val :=
-  let b' := rev_if_be _ b in
-  match (proj_int wz b') with
-  | Some i => Vint wz i
-  | None => Vundef
-  end.
+Definition decode_int (wz:nat) (b: list byte) : Int.int wz :=
+  let b' := rev_if_be _ b in Int.repr wz (int_of_bytes b').
+
+Definition decode_float32 (b: list byte) : Int.int 31 := Int.zero 31.
+
+Definition decode_float64 (b: list byte) : Int.int 63 := Int.zero 63.
 
 Lemma encode_int_length:
-  forall wz n, length(encode_int wz n) = bytesize_chunk_nat wz.
+  forall chunk wz x, length (encode_int chunk wz x) = size_chunk_nat chunk.
 Proof.
   intros. unfold encode_int. rewrite rev_if_be_length.
-  apply length_inj_int.
+  destruct chunk; rewrite length_bytes_of_int; reflexivity.
 Qed.
 
-Lemma decode_encode_int_eq:
-  forall wz x,
-  decode_int (encode_int wz x) wz = Vint wz x.
+Lemma decode_encode_int:
+  forall c wz x,
+  match c with
+  | Mint wz0 => 
+      decode_int wz0 (encode_int c wz x) = Int.repr wz0 (Int.unsigned wz x)
+  | Mfloat32 => decode_float32 (encode_int c wz x) = Int.zero 31
+  | Mfloat64 => decode_float64 (encode_int c wz x) = Int.zero 63
+  end.
 Proof.
-  intros. unfold decode_int, encode_int; auto;
-  rewrite rev_if_be_involutive.
+  intros. 
+  unfold decode_int, encode_int, decode_float32, decode_float64; destruct c; 
+  auto; rewrite rev_if_be_involutive.
 
-  rewrite proj_inj_int_eq. auto.
-Qed.
+  rewrite int_of_bytes_of_int.
+  assert (J:=@bytesize_chunk_pos n).
+  rewrite nat_of_Z_eq; try omega.
+  apply Int.eqm_samerepr. 
+  unfold Int.eqm, Int.eqmod.
+  unfold Int.modulus.
+  unfold Int.wordsize.
+  unfold bytesize_chunk.  
+  assert (8 > 0) as J'. omega.
+  assert (J1:=@ZRdiv_prop1 (Z_of_nat (S n)) 8 J').
+  assert (8 * ZRdiv (Z_of_nat (S n)) 8 = ZRdiv (Z_of_nat (S n)) 8 * 8) as EQ.
+    auto with zarith.
+  rewrite EQ in J1. clear EQ.
+  assert (J2:=Z_of_S_gt_O n).
+  assert (two_power_nat (S n) = two_p (Z_of_nat (S n))) as EQ.
+    simpl.
+    rewrite two_power_pos_nat.
+    rewrite S_eq_nat_of_P_o_P_of_succ_nat. auto.
 
-Lemma decode_encode_int_neq:
-  forall wz1 wz2 x,
-  wz1 <> wz2 ->
-  decode_int (encode_int wz1 x) wz2 = Vundef.
-Proof.
-  intros. unfold decode_int, encode_int; auto;
-  rewrite rev_if_be_involutive.
+  rewrite EQ. clear EQ.
+  (* 
+     let m1 = ZRdiv (Z_of_nat (S n)) 8 * 8
+     let m2 = S n
+     x % (2^m1) = 2^m1 * k0 + x for some k0
+     so,
+     x % (2^m1) = 2^m2 * (2^(m1-m2) * k0) + x
+     so (2^(m1-m2) * k0) is the witness
+  *) 
+  remember (ZRdiv (Z_of_nat (S n)) 8 * 8) as m1.
+  remember (Z_of_nat (S n)) as m2.    
+  rewrite Zmod_eq with (a:=Int.unsigned wz x) (b:=two_p m1).
+    remember (Int.unsigned wz x / two_p m1) as k0.
+    exists ( - two_p (m1 - m2) * k0).
+    ring_simplify.
+    rewrite <- Zmult_assoc.
+    rewrite <- two_p_is_exp; auto with zarith.
+    assert (m1 = m1 - m2 + m2) as EQ. auto with zarith.
+    rewrite <- EQ. clear EQ.
+    auto.
 
-  rewrite proj_inj_int_neq; auto.
-Qed.
-
-Remark encode_mod:
-  forall wz x y, 
-  Int.eqmod (two_p (wordsize_chunk wz)) (Int.unsigned wz x) (Int.unsigned wz y) ->
-  encode_int wz x = encode_int wz y.
-Proof.
-  intros. unfold encode_int. decEq.
-  unfold inj_int.
-  unfold wordsize_chunk in H. 
-  unfold bytesize_chunk in H.
-  apply bytes_of_int_mod' in H; try solve [apply ZRdiv_prop4].
-  rewrite H. auto.
+    apply two_p_gt_ZERO. auto with zarith.
 Qed.
 
 (** * Encoding and decoding floats *)
@@ -690,7 +585,47 @@ Qed.
 
 (** * Encoding and decoding values *)
 
-Fixpoint inj_pointer (n: nat) (b: block) (ofs: Int.int 31) {struct n}: list memval :=
+Definition inj_bytes (wz:nat) (bl: list byte) : list memval :=
+  List.map (Byte wz) bl.
+
+Fixpoint proj_bytes (wz:nat) (vl: list memval) : option (list byte) :=
+  match vl with
+  | nil => Some nil
+  | Byte wz0 b :: vl' =>
+      if eq_nat_dec wz0 wz then
+        match proj_bytes wz vl' with None => None | Some bl => Some(b :: bl) end
+      else None
+  | _ => None
+  end.
+
+Remark length_inj_bytes:
+  forall wz bl, length (inj_bytes wz bl) = length bl.
+Proof.
+  intros. apply List.map_length.
+Qed.
+
+Remark proj_inj_bytes:
+  forall wz bl, proj_bytes wz (inj_bytes wz bl) = Some bl.
+Proof.
+  induction bl; simpl; auto. 
+    rewrite IHbl.
+    destruct (eq_nat_dec wz wz); auto.
+      contradict n; auto.
+Qed.
+
+Lemma inj_proj_bytes:
+  forall wz cl bl, proj_bytes wz cl = Some bl -> cl = inj_bytes wz bl.
+Proof.
+  induction cl; simpl; intros.
+  inv H; auto.
+  destruct a; try congruence.
+  destruct (eq_nat_dec n wz); try solve [inv H].
+  destruct (proj_bytes wz cl); inv H.
+  simpl. decEq. auto.
+Qed.
+
+Fixpoint inj_pointer (n: nat) (b: block) (ofs: Int.int 31) {struct n} 
+  : list memval :=
   match n with
   | O => nil
   | S m => Pointer b ofs m :: inj_pointer m b ofs
@@ -701,7 +636,8 @@ Fixpoint check_pointer (n: nat) (b: block) (ofs: Int.int 31) (vl: list memval)
   match n, vl with
   | O, nil => true
   | S m, Pointer b' ofs' m' :: vl' =>
-      eq_block b b' && Int.eq_dec 31 ofs ofs' && beq_nat m m' && check_pointer m b ofs vl'
+      eq_block b b' && Int.eq_dec 31 ofs ofs' && beq_nat m m' && 
+      check_pointer m b ofs vl'
   | _, _ => false
   end.
 
@@ -766,71 +702,60 @@ Proof.
   rewrite <- beq_nat_refl. simpl; auto.
 Qed.
 
+Definition wz_of_chunk (chunk: memory_chunk) : nat :=
+  match chunk with
+  | Mint wz => wz
+  | Mfloat32 => 31%nat
+  | Mfloat64 => 63%nat
+  end.
+  
 Definition encode_val (chunk: memory_chunk) (v: val) : list memval :=
   match v, chunk with
   | Vptr b ofs, Mint wz => 
-    if eq_nat_dec wz 31 
-    then inj_pointer (size_chunk_nat (Mint wz)) b ofs
-    else list_repeat (size_chunk_nat chunk) Undef
+      if (eq_nat_dec wz 31) then inj_pointer (size_chunk_nat (Mint32)) b ofs
+      else list_repeat (size_chunk_nat chunk) Undef
   | Vinttoptr i, Mint wz => 
-    if eq_nat_dec wz 31 
-    then inj_ipointer (size_chunk_nat (Mint wz)) i
-    else list_repeat (size_chunk_nat chunk) Undef
-  | Vint wz n, Mint wz' =>
-    if eq_nat_dec wz wz' 
-    then encode_int wz n
-    else list_repeat (size_chunk_nat chunk) Undef
-  | Vfloat f, _ => inj_bytes (encode_float chunk f)
+      if (eq_nat_dec wz 31) then inj_ipointer (size_chunk_nat (Mint wz)) i
+      else list_repeat (size_chunk_nat chunk) Undef
+  | Vint wz n, _ => inj_bytes (wz_of_chunk chunk) (encode_int chunk wz n)
+  | Vfloat f, _ => inj_bytes (wz_of_chunk chunk) (encode_float chunk f)
   | _, _ => list_repeat (size_chunk_nat chunk) Undef
   end.
 
 Definition decode_val (chunk: memory_chunk) (vl: list memval) : val :=
-  match chunk with
-  | Mint wz => 
-    match decode_int vl wz with
-    | Vundef => 
-        if eq_nat_dec wz 31 then 
-          match proj_pointer vl with
-          | Vundef => proj_ipointer vl
-          | v => v
-          end
-        else Vundef
-    | v => v
-    end
-  | Mfloat32 =>
-    match proj_bytes (bytesize_chunk_nat 31) vl with
-    | Some bl => Vfloat(decode_float chunk bl)
-    | None => Vundef
-    end
-  | Mfloat64 =>
-    match proj_bytes (bytesize_chunk_nat 63) vl with
-    | Some bl => Vfloat(decode_float chunk bl)
-    | None => Vundef
-    end
+  match proj_bytes (wz_of_chunk chunk) vl with
+  | Some bl =>
+      match chunk with
+      | Mint _ => Vint (wz_of_chunk chunk) (decode_int (wz_of_chunk chunk) bl)
+      | Mfloat32 | Mfloat64 => Vfloat(decode_float chunk bl)
+      end
+  | None =>
+      match chunk with
+      | Mint wz => 
+          if eq_nat_dec wz 31 then
+            match proj_pointer vl with
+            | Vundef => proj_ipointer vl
+            | v => v
+            end
+          else Vundef 
+      | _ => Vundef
+      end
   end.
 
 Lemma encode_val_length:
-  forall chunk v, length (encode_val chunk v) = size_chunk_nat chunk.
+  forall chunk v, length(encode_val chunk v) = size_chunk_nat chunk.
 Proof.
   intros. destruct v; simpl.
-
   apply length_list_repeat.
-
-  destruct chunk; simpl; unfold size_chunk_nat, size_chunk; auto with zarith.
-  destruct (eq_nat_dec wz n); subst.
-    apply encode_int_length.
-    apply length_list_repeat.
-
+  rewrite length_inj_bytes. apply encode_int_length.
   rewrite length_inj_bytes. apply encode_float_length.
 
-  destruct chunk; simpl; unfold size_chunk_nat, size_chunk; auto.
-    destruct (eq_nat_dec n 31); subst.
-      apply inj_pointer_length.
+  destruct chunk; try (apply length_list_repeat). 
+    destruct (eq_nat_dec n 31); subst; auto.
       apply length_list_repeat.
 
-  destruct chunk; simpl; unfold size_chunk_nat, size_chunk; auto.
-    destruct (eq_nat_dec n 31); subst.
-      apply inj_ipointer_length.
+  destruct chunk; try (apply length_list_repeat). 
+    destruct (eq_nat_dec n 31); subst; auto.
       apply length_list_repeat.
 Qed.
 
@@ -838,59 +763,91 @@ Definition decode_encode_val (v1: val) (chunk1 chunk2: memory_chunk) (v2: val)
   : Prop :=
   match v1, chunk1, chunk2 with
   | Vundef, _, _ => v2 = Vundef
-
   | Vint wz n, Mint wz1, Mint wz2 => 
-    if eq_nat_dec wz wz1
-    then 
-      if eq_nat_dec wz wz2
-      then v2 = Vint wz n
-      else v2 = Vundef
-    else v2 = Vundef
-  | Vint wz n, Mint wz', Mfloat32 => 
-    if eq_nat_dec wz 31
-    then 
-      if eq_nat_dec wz' 31
-      then 
-        match (proj_bytes (bytesize_chunk_nat wz) (encode_int wz n)) with
-        | Some bl => v2 = Vfloat(decode_float Mfloat32 bl)
-        | None => False
-        end
+      if eq_nat_dec wz1 wz2 then 
+        v2 = Vint wz2 (Int.repr wz2 (Int.unsigned wz n)) 
       else True
-    else True
+  | Vint wz n, Mint wz', Mfloat32 => 
+      if eq_nat_dec wz' 31
+      then v2 = Vfloat(decode_float Mfloat32 (encode_int (Mint32) wz n))
+      else True
   | Vint wz n, _, _ => True   (* nothing interesting to say about v2 *)
-
   | Vptr b ofs, Mint wz1, Mint wz2 => 
-    if eq_nat_dec wz1 31
-    then 
-      if eq_nat_dec wz2 31
-      then v2 = Vptr b ofs
-      else v2 = Vundef
-    else v2 = Vundef
+      if eq_nat_dec wz1 31 && eq_nat_dec wz2 31 
+      then v2 = Vptr b ofs else v2 = Vundef
   | Vptr b ofs, _, _ => v2 = Vundef
-
   | Vinttoptr i, Mint wz1, Mint wz2 => 
-    if eq_nat_dec wz1 31
-    then 
-      if eq_nat_dec wz2 31
-      then v2 = Vinttoptr i
-      else v2 = Vundef
-    else v2 = Vundef
+      if eq_nat_dec wz1 31 && eq_nat_dec wz2 31
+      then v2 = Vinttoptr i else v2 = Vundef
   | Vinttoptr i, _, _ => v2 = Vundef
-
   | Vfloat f, Mfloat32, Mfloat32 => v2 = Vfloat(Float.singleoffloat f)
   | Vfloat f, Mfloat32, Mint wz => 
-    if eq_nat_dec wz 31
-    then v2 = decode_int (inj_bytes (encode_float Mfloat32 f)) 31
-    else True
+      if eq_nat_dec wz 31
+      then v2 = Vint 31 (decode_int 31 (encode_float Mfloat32 f))
+      else True
   | Vfloat f, Mfloat64, Mfloat64 => v2 = Vfloat f
   | Vfloat f, _, _ => True   (* nothing interesting to say about v2 *)
   end.
 
-Remark proj_bytes_undef:
-  forall n, (n > 0)%nat -> proj_bytes n (list_repeat n Undef) = None.
+Lemma proj_bytes_inj_pointer:
+  forall wz n b i, (n > 0)%nat -> proj_bytes wz (inj_pointer n b i) = None.
 Proof.
-  induction n; simpl; intro; auto.
+  induction n; simpl; auto. 
+    intros. contradict H; omega.
+Qed.
+
+Lemma inj_pointer_inv : forall n b i,
+  (n > 0)%nat -> 
+  exists m, exists tl, inj_pointer n b i = Pointer b i m :: tl /\ n = S m.
+Proof.
+  destruct n; intros.
     contradict H; omega.
+    simpl. exists n. exists (inj_pointer n b i). auto.
+Qed.
+
+Lemma bytesize_chunk_nat__size_chunk_nat : forall n,
+  size_chunk_nat (Mint n) = bytesize_chunk_nat n.
+Proof.
+  intros. 
+  unfold size_chunk_nat, bytesize_chunk_nat, size_chunk, bytesize_chunk.
+  auto.
+Qed.
+
+Lemma list_repeat_cons_inv : forall A m (a:A) b v,
+  a :: b = list_repeat m v ->
+  a = v /\
+  exists m', S m' = m /\ b = list_repeat m' v.
+Proof.
+  induction m; intros; simpl in *.
+    inversion H.
+
+    inversion H; subst.
+    split; auto.
+    exists m. split; auto.
+Qed.
+
+Lemma nonempty_list_repeat : forall A m (v:A),
+  (m > 0)%nat -> nil <> list_repeat m v.
+Proof.
+  induction m; simpl; intros.
+    contradict H; omega.
+    intro J. inversion J.
+Qed.
+
+Lemma proj_bytes_undef' : forall n m,
+  (m > 0)%nat ->
+  proj_bytes n (list_repeat m Undef) = None.
+Proof.
+  intros.
+  remember (list_repeat m Undef) as L.
+  generalize dependent m.
+  generalize dependent n.
+  induction L; intros; simpl.
+    contradict HeqL.
+    apply nonempty_list_repeat; auto.
+
+    apply list_repeat_cons_inv in HeqL.
+    destruct HeqL as [H1 [m' [H2 H3]]]; subst; auto.
 Qed.
 
 Remark proj_pointer_undef':
@@ -905,145 +862,38 @@ Proof.
   induction n; simpl; auto.
 Qed.
 
-Lemma list_repeat_cons_inv : forall m a b,
-  a :: b = list_repeat m Undef ->
-  a = Undef /\
-  exists m', S m' = m /\ b = list_repeat m' Undef.
-Proof.
-  induction m; intros; simpl in *.
-    inversion H.
-
-    inversion H; subst.
-    split; auto.
-    exists m. split; auto.
-Qed.
-
-Lemma proj_int_undef : forall n m,
-  proj_int n (list_repeat m Undef) = None.
+Lemma proj_pointer_inj_pointer:
+  forall b i, proj_pointer (inj_pointer (size_chunk_nat Mint32) b i) = Vptr b i.
 Proof.
   intros.
-  unfold proj_int.
-  remember (nat_of_Z (ZRdiv (Z_of_nat (S n)) 8)) as N.
-  induction N; simpl.
-    destruct (list_repeat m Undef); auto.
-
-    remember (list_repeat m Undef) as L.
-    destruct L; auto.
-      apply list_repeat_cons_inv in HeqL.
-      destruct HeqL as [H1 [m' [H2 H3]]]; subst; auto.
-Qed.      
-
-Lemma list_repeat_undef : forall n,
-  list_repeat n Undef ++ Undef :: nil =
-  Undef :: list_repeat n Undef.
-Proof.
-  induction n; simpl; auto.
-    rewrite IHn. auto.
+  Opaque check_pointer. 
+  simpl.
+  rewrite check_inj_pointer. auto.
+  Transparent check_pointer. 
 Qed.
 
-Lemma rev_if_be_nil : forall (A:Type), rev_if_be A nil = nil.
+Lemma proj_bytes_inj_ipointer:
+  forall wz n i, (n > 0)%nat -> proj_bytes wz (inj_ipointer n i) = None.
 Proof.
-  unfold rev_if_be.
-  destruct big_endian; auto.
+  induction n; simpl; intros; auto. 
+    contradict H; omega.
 Qed.
 
-Lemma rev_if_be_repeat_undef : forall n,
-  rev_if_be _ (list_repeat n Undef) = list_repeat n Undef.
+Lemma proj_pointer_inj_ipointer:
+  forall i, proj_pointer (inj_ipointer (size_chunk_nat Mint32) i) = Vundef.
 Proof.
-  induction n; simpl.
-    apply rev_if_be_nil.
-
-    unfold rev_if_be in *.
-    destruct big_endian; auto.
-      simpl.
-      rewrite IHn. auto.
-      apply list_repeat_undef.
+  intros. simpl. auto.
 Qed.
 
-Lemma proj_pointer_encode_int : forall wz i,
-  proj_pointer (encode_int wz i) = Vundef.
+Lemma proj_ipointer_inj_ipointer:
+  forall i, proj_ipointer (inj_ipointer (size_chunk_nat Mint32) i) = Vinttoptr i.
 Proof.
   intros.
-  unfold proj_pointer, encode_int, inj_int.
-  destruct (bytes_of_int (nat_of_Z (ZRdiv (Z_of_nat (S wz)) 8)) 
-                         (Int.unsigned wz i)); simpl; auto.
-    rewrite rev_if_be_nil. auto.
-Admitted.
-
-Lemma proj_ipointer_encode_int : forall wz i,
-  proj_ipointer (encode_int wz i) = Vundef.
-Proof.
-  intros.
-  unfold proj_ipointer, encode_int, inj_int.
-  destruct (bytes_of_int (nat_of_Z (ZRdiv (Z_of_nat (S wz)) 8)) 
-                         (Int.unsigned wz i)); simpl; auto.
-    rewrite rev_if_be_nil. auto.
-Admitted.
-
-Lemma decode_int_repeat_Undef : forall n m,
-  decode_int (list_repeat n Undef) m = Vundef.
-Proof.
-  intros.
-  unfold decode_int.
-  rewrite rev_if_be_repeat_undef.
-  rewrite proj_int_undef. auto.
+  Opaque check_ipointer. 
+  simpl.
+  rewrite check_inj_ipointer. auto.
+  Transparent check_ipointer. 
 Qed.
-
-Lemma proj_bytes_encode_int32 : forall i,
-  exists bl, proj_bytes (bytesize_chunk_nat 31) (encode_int 31 i) = Some bl.
-Admitted.
-
-Lemma decode_int_encode_float32 : forall f,
-  exists i, decode_int (inj_bytes (encode_float Mfloat32 f)) 31 = Vint 31 i.
-Admitted.
-
-Lemma proj_bytes_encode_float32 : forall f,
-  exists bl, proj_bytes (bytesize_chunk_nat 31) (inj_bytes (encode_float Mfloat32 f)) = Some bl.
-Admitted.      
-
-Lemma proj_bytes_encode_float64 : forall f,
-  exists bl, proj_bytes (bytesize_chunk_nat 63) (inj_bytes (encode_float Mfloat64 f)) = Some bl.
-Admitted.      
-
-Lemma encode_float32_length : forall f,
-  length (encode_float Mfloat32 f) = bytesize_chunk_nat 31.
-Admitted.
-
-Lemma encode_float64_length : forall f,
-  length (encode_float Mfloat64 f) = bytesize_chunk_nat 63.
-Admitted.
-
-Lemma decode_int_inj_pointer:
-  forall b ofs, 
-  decode_int (inj_pointer (size_chunk_nat Mint32) b ofs) 31 = Vptr b ofs.
-Proof.
-Admitted.
-
-Lemma decode_int_inj_pointer_undef:
-  forall b ofs n, 
-  n <> 31%nat ->
-  decode_int (inj_pointer (size_chunk_nat Mint32) b ofs) n = Vundef.
-Proof.
-Admitted.
-
-Lemma decode_int_inj_ipointer:
-  forall i, 
-  decode_int (inj_ipointer (size_chunk_nat Mint32) i) 31 = Vinttoptr i.
-Proof.
-Admitted.
-
-Lemma decode_int_inj_ipointer_undef:
-  forall i n, 
-  n <> 31%nat ->
-  decode_int (inj_ipointer (size_chunk_nat Mint32) i) n = Vundef.
-Proof.
-Admitted.
-
-Remark proj_bytes_undef':
-  forall n m, (m > 0)%nat -> proj_bytes n (list_repeat m Undef) = None.
-Proof.
-  induction n; simpl; intros; auto.
-Admitted.
 
 Lemma decode_encode_val_general:
   forall v chunk1 chunk2,
@@ -1051,113 +901,71 @@ Lemma decode_encode_val_general:
 Proof.
   intros. destruct v.
 (* Vundef *)
-  simpl. destruct (size_chunk_nat_pos chunk1) as [psz EQ]. 
+  simpl. destruct (size_chunk_nat_pos chunk1) as [psz EQ].
   rewrite EQ. simpl.
-  unfold decode_val. simpl. destruct chunk2; auto.
-  change (Undef::list_repeat psz Undef) with (list_repeat (S psz) Undef).
-  rewrite decode_int_repeat_Undef.
-  destruct (eq_nat_dec n 31); subst; auto.
+  unfold decode_val. simpl. 
+  destruct chunk2; auto.
+  destruct (eq_nat_dec n 31); auto.
 (* Vint *)
   simpl.
-  destruct chunk1; auto; destruct chunk2; auto; unfold decode_val, encode_val; 
-  try rewrite proj_inj_bytes.
+  destruct chunk1; auto; destruct chunk2; auto; unfold decode_val; simpl.
+    destruct (eq_nat_dec n n0); subst; simpl; auto.
+      rewrite proj_inj_bytes.
+      rewrite decode_encode_int with (c:=Mint n0). auto.
 
-    destruct (eq_nat_dec wz n); subst; auto.
-      destruct (eq_nat_dec n n0); subst; auto.
-        rewrite decode_encode_int_eq; auto.
-        rewrite decode_encode_int_neq; auto.
-        destruct (eq_nat_dec n0 31); subst; auto.
-          rewrite proj_pointer_encode_int.
-          apply proj_ipointer_encode_int.
-      rewrite decode_int_repeat_Undef.
-      destruct (eq_nat_dec n0 31); subst; auto.
-        rewrite proj_pointer_undef'.
-        apply proj_ipointer_undef'.
-      
-    destruct (eq_nat_dec wz 31); subst; auto.
-      destruct (eq_nat_dec n 31); subst; auto.
-        destruct (eq_nat_dec 31 31); subst.
-          destruct (@proj_bytes_encode_int32 i) as [bl EQ].
-          rewrite EQ.
-          simpl. auto.
-          
-          contradict n; auto.
+    destruct (eq_nat_dec n 31); subst; auto.
+    rewrite proj_inj_bytes. auto.
 (* Vfloat *)
   unfold decode_val, encode_val, decode_encode_val;
   destruct chunk1; auto; destruct chunk2; auto; unfold decode_val.
-
     destruct (eq_nat_dec n 31); subst; auto.
-      destruct (@decode_int_encode_float32 f) as [i EQ].
-      rewrite EQ. auto.
+    rewrite proj_inj_bytes. auto.
 
-      destruct (@proj_bytes_encode_float32 f) as [bl EQ].
-      rewrite EQ. simpl.
-      decEq.
-      rewrite <- decode_encode_float32.
-      unfold decode_float.
-      rewrite <- (encode_float32_length f) in EQ.
-      rewrite proj_inj_bytes in EQ.
-      inversion EQ; subst; auto.
+    rewrite proj_inj_bytes. 
+    rewrite decode_encode_float32. auto.
 
-    destruct (@proj_bytes_encode_float64 f) as [bl EQ].
-    rewrite EQ. simpl.
-    decEq.
-    rewrite <- decode_encode_float64.
-    unfold decode_float.
-    rewrite <- (encode_float64_length f) in EQ.
-    rewrite proj_inj_bytes in EQ.
-    inversion EQ; subst; auto.
-
+    rewrite proj_inj_bytes. 
+    rewrite decode_encode_float64. auto.
 (* Vptr *)
+  assert (J:=@size_chunk_nat_pos' chunk1).
   unfold decode_val, encode_val, decode_encode_val;
   destruct chunk1; auto; destruct chunk2; auto.
-
     destruct (eq_nat_dec n 31); subst; auto.
-      destruct (eq_nat_dec n0 31); subst; auto.
-        rewrite decode_int_inj_pointer; auto.
-        rewrite decode_int_inj_pointer_undef; auto.
-
-      rewrite decode_int_repeat_Undef.
-      destruct (eq_nat_dec n0 31); subst; auto.
-        rewrite proj_pointer_undef'; auto.
-        rewrite proj_ipointer_undef'; auto.
-
+      rewrite proj_bytes_inj_pointer; auto using size_chunk_nat_pos'.
+      rewrite proj_pointer_inj_pointer.
+      destruct (eq_nat_dec n0 31); subst; simpl; auto.
+ 
+      simpl. rewrite proj_bytes_undef'; auto. rewrite proj_pointer_undef'.
+      rewrite proj_ipointer_undef'.
+      destruct (eq_nat_dec n0 31); subst; simpl; auto.
     destruct (eq_nat_dec n 31); subst; auto.
-      rewrite proj_bytes_undef'; auto using size_chunk_nat_pos'.
-
+       rewrite proj_bytes_undef'; auto. 
     destruct (eq_nat_dec n 31); subst; auto.
-      rewrite proj_bytes_undef'; auto using size_chunk_nat_pos'.
-
-    rewrite decode_int_repeat_Undef.
+      rewrite proj_bytes_undef'; auto. 
+    rewrite proj_bytes_undef'; auto.
     destruct (eq_nat_dec n 31); subst; auto.
-   
-    rewrite decode_int_repeat_Undef.
+    rewrite proj_bytes_undef'; auto.
     destruct (eq_nat_dec n 31); subst; auto.
-
-(* Vinttoptr *)
+(* Vint2ptr *)
+  assert (J:=@size_chunk_nat_pos' chunk1).
   unfold decode_val, encode_val, decode_encode_val;
   destruct chunk1; auto; destruct chunk2; auto.
-
     destruct (eq_nat_dec n 31); subst; auto.
-      destruct (eq_nat_dec n0 31); subst; auto.
-        rewrite decode_int_inj_ipointer; auto.
-        rewrite decode_int_inj_ipointer_undef; auto.
-
-      rewrite decode_int_repeat_Undef.
-      destruct (eq_nat_dec n0 31); subst; auto.
-        rewrite proj_pointer_undef'; auto.
-        rewrite proj_ipointer_undef'; auto.
-
+      rewrite proj_bytes_inj_ipointer; auto using size_chunk_nat_pos'.
+      rewrite proj_pointer_inj_ipointer.
+      rewrite proj_ipointer_inj_ipointer.
+      destruct (eq_nat_dec n0 31); subst; simpl; auto.
+ 
+      simpl. rewrite proj_bytes_undef'; auto. rewrite proj_pointer_undef'.
+      rewrite proj_ipointer_undef'.
+      destruct (eq_nat_dec n0 31); subst; simpl; auto.
     destruct (eq_nat_dec n 31); subst; auto.
-      rewrite proj_bytes_undef'; auto using size_chunk_nat_pos'.
-
+       rewrite proj_bytes_undef'; auto. 
     destruct (eq_nat_dec n 31); subst; auto.
-      rewrite proj_bytes_undef'; auto using size_chunk_nat_pos'.
-
-    rewrite decode_int_repeat_Undef.
+      rewrite proj_bytes_undef'; auto. 
+    rewrite proj_bytes_undef'; auto.
     destruct (eq_nat_dec n 31); subst; auto.
-   
-    rewrite decode_int_repeat_Undef.
+    rewrite proj_bytes_undef'; auto.
     destruct (eq_nat_dec n 31); subst; auto.
 Qed.
 
@@ -1169,42 +977,33 @@ Lemma decode_encode_val_similar:
   decode_encode_val v1 chunk1 chunk2 v2 ->
   v2 = Val.load_result chunk2 v1.
 Proof.
-  intros. 
+  intros.
   destruct v1.
   simpl in *. destruct chunk2; simpl; auto.
- 
+
   red in H1.
   destruct chunk1; simpl in H1; try contradiction;
   destruct chunk2; simpl in *; discriminate || auto.
-  destruct (eq_nat_dec wz n); subst.
-    destruct (eq_nat_dec n n0); subst.
-      destruct (eq_nat_dec n0 n0); subst; auto.
-        contradict n; auto.
-      destruct (eq_nat_dec n0 n); subst; auto.
-        contradict n1; auto.
-    destruct (eq_nat_dec n0 wz); subst; auto.
-      unfold chunk_eq in H0.
-      destruct H0; subst.
-      contradict n1; auto.
+  unfold chunk_eq in H0. destruct H0; subst.
+  destruct (eq_nat_dec n0 n0); auto.
+    contradict n; auto.
 
   unfold chunk_eq in H0. destruct H0.
   red in H1.
   destruct chunk1; simpl in H1; try contradiction;
   destruct chunk2; simpl in *; discriminate || auto.
-    
+
   unfold chunk_eq in H0. destruct H0.
   red in H1.
   destruct chunk1; simpl in H1; try contradiction;
   destruct chunk2; simpl in *; discriminate || auto.
-  subst.
-  destruct (eq_nat_dec n0 31); subst; auto.
-    
+  subst. destruct (eq_nat_dec n0 31); auto.
+
   unfold chunk_eq in H0. destruct H0.
   red in H1.
   destruct chunk1; simpl in H1; try contradiction;
   destruct chunk2; simpl in *; discriminate || auto.
-  subst.
-  destruct (eq_nat_dec n0 31); subst; auto.
+  subst. destruct (eq_nat_dec n0 31); auto.
 Qed.
 
 Lemma decode_val_type:
@@ -1214,19 +1013,19 @@ Proof.
   intros. unfold decode_val.
   destruct chunk; simpl; auto. 
 
-    unfold decode_int.
-    destruct (proj_int n (rev_if_be memval cl)); simpl; auto.
+    unfold decode_int.    
+    destruct (proj_bytes n cl); simpl; auto.
       destruct (eq_nat_dec n 31); simpl; auto.
-        unfold proj_pointer.
-        destruct cl; simpl; auto.
-          destruct m; simpl; auto.
+        unfold proj_pointer. unfold proj_ipointer.
+        destruct cl; try solve [simpl; auto].
+          destruct m; try solve [simpl; auto].
             destruct (check_pointer (size_chunk_nat Mint32) b i 
-                       (Pointer b i n0::cl)); simpl; auto.
+                       (Pointer b i n0::cl)); simpl; auto.            
             destruct (check_ipointer (size_chunk_nat Mint32) i 
                        (IPointer i n0::cl)); simpl; auto.
 
-    destruct (proj_bytes (bytesize_chunk_nat 31) cl); simpl; auto.
-    destruct (proj_bytes (bytesize_chunk_nat 63) cl); simpl; auto.
+    destruct (proj_bytes 31 cl); simpl; auto.
+    destruct (proj_bytes 63 cl); simpl; auto.
 Qed.
 
 (*
@@ -1268,89 +1067,62 @@ Qed.
 *)
 
 Lemma decode_val_int_inv:
-  forall chunk cl n i,
-  decode_val chunk cl = Vint n i ->
+  forall chunk cl n,
+  decode_val chunk cl = Vint (wz_of_chunk chunk) n ->
   type_of_chunk chunk = Tint /\
-  Vint n i = decode_int cl n.
+  exists bytes, proj_bytes (wz_of_chunk chunk) cl = Some bytes /\ 
+    n = decode_int (wz_of_chunk chunk) bytes.
 Proof.
-  intros until i. unfold decode_val.
-  destruct chunk; intro EQ.
-    remember (decode_int cl n0) as R.
-    unfold decode_int in HeqR.
-    remember (proj_int n0 (rev_if_be memval cl)) as R'.
-    split. simpl. auto.
-      unfold decode_int.
-      destruct R'; subst.
-        inversion EQ; subst.
-        rewrite <- HeqR'. auto.
+  intros until n. unfold decode_val. 
+  destruct (proj_bytes (wz_of_chunk chunk) cl).
+Opaque decode_int.
+    destruct chunk; intro EQ; inv EQ; split; auto; exists l; auto.
 
-        destruct (eq_nat_dec n0 31); subst; try solve [inversion EQ].
-          unfold proj_pointer in EQ.
-          destruct cl; try solve [inversion EQ].
-          destruct m; try solve [inversion EQ].
-          destruct (check_pointer (size_chunk_nat Mint32) b i0 
-            (Pointer b i0 n0::cl)); try solve [inversion EQ].
-
-          unfold proj_ipointer in EQ.
-          destruct (check_ipointer (size_chunk_nat Mint32) i0 
-            (IPointer i0 n0::cl)); try solve [inversion EQ].
-
-    destruct (proj_bytes (bytesize_chunk_nat 31) cl); subst; 
-      try solve [inversion EQ].
-    destruct (proj_bytes (bytesize_chunk_nat 63) cl); subst; 
-      try solve [inversion EQ].
+    destruct chunk; try congruence. 
+    destruct (eq_nat_dec n0 31); subst; try congruence. 
+    unfold proj_pointer, proj_ipointer.
+    destruct cl; try congruence. 
+    destruct m; try congruence.
+      destruct (check_pointer (size_chunk_nat Mint32) b i 
+        (Pointer b i n0 :: cl)); congruence.
+      destruct (check_ipointer (size_chunk_nat Mint32) i 
+        (IPointer i n0 :: cl)); congruence.
 Qed.
 
 Lemma decode_val_float_inv:
   forall chunk cl f,
   decode_val chunk cl = Vfloat f ->
   type_of_chunk chunk = Tfloat /\
-  exists bl, 
-    proj_bytes (size_chunk_nat chunk) cl = Some bl /\ f = decode_float chunk bl.
+  exists bytes, proj_bytes (wz_of_chunk chunk) cl = Some bytes /\ 
+    f = decode_float chunk bytes.
 Proof.
   intros until f. unfold decode_val. 
-  destruct chunk; intro EQ.
-    remember (decode_int cl n) as R.
-    unfold decode_int in HeqR.
-    remember (proj_int n (rev_if_be memval cl)) as R'.
-    destruct R'; subst; try solve [inversion EQ].
-      destruct (eq_nat_dec n 31); subst; try solve [inversion EQ].
-        unfold proj_pointer in EQ.
-        destruct cl; try solve [inversion EQ].
-        destruct m; try solve [inversion EQ].
-        destruct (check_pointer (size_chunk_nat Mint32) b i (Pointer b i n::cl));
-          try solve [inversion EQ].
+  destruct (proj_bytes (wz_of_chunk chunk) cl).
+    destruct chunk; intro EQ; inv EQ; split; auto; exists l; auto.
 
-        unfold proj_ipointer in EQ.
-        destruct (check_ipointer (size_chunk_nat Mint32) i (IPointer i n::cl));
-          try solve [inversion EQ].
-
-    remember (proj_bytes (bytesize_chunk_nat 31) cl) as R.
-    destruct R; subst; try solve [inversion EQ].
-    split; auto.
-      unfold decode_float in EQ.
-      inversion EQ; subst.
-      exists l. split; auto.
-
-    remember (proj_bytes (bytesize_chunk_nat 63) cl) as R.
-    destruct R; subst; try solve [inversion EQ].
-    split; auto.
-      unfold decode_float in EQ.
-      inversion EQ; subst.
-      exists l. split; auto.
+    destruct chunk; try congruence.
+    destruct (eq_nat_dec n 31); subst; try congruence.
+    unfold proj_pointer. unfold proj_ipointer.
+    destruct cl; try congruence. 
+    destruct m; try congruence.
+      destruct (check_pointer (size_chunk_nat Mint32) b i (Pointer b i n :: cl));
+        congruence.
+      destruct (check_ipointer (size_chunk_nat Mint32) i (IPointer i n :: cl));
+        congruence.
 Qed.
 
 Lemma decode_val_cast:
   forall chunk l,
   let v := decode_val chunk l in
   match chunk with
+  | Mint wz => True
   | Mfloat32 => v = Val.singleoffloat v
   | _ => True
   end.
 Proof.
-  unfold decode_val; intros; destruct chunk; auto; 
-    destruct (proj_bytes (bytesize_chunk_nat 31) l); auto.
-  unfold Val.singleoffloat. decEq. symmetry. apply decode_float32_cast. 
+  unfold decode_val; intros; destruct chunk; auto.
+  destruct (proj_bytes (wz_of_chunk Mfloat32) l); auto.
+  unfold Val.singleoffloat. decEq. symmetry. apply decode_float32_cast.
 Qed.
 
 (** Pointers cannot be forged. *)
@@ -1375,108 +1147,35 @@ Inductive encoding_shape: list memval -> Prop :=
       (forall mv, In mv mvl -> memval_valid_cont mv) ->
       encoding_shape (mv1 :: mvl).
 
-Lemma encoding_shape_undef : forall n,
-  (n > 0)%nat ->
-  encoding_shape (list_repeat n Undef).
-Proof.
-  induction n; intros.
-    contradict H; omega.
-
-    simpl.
-    apply encoding_shape_intro.
-      simpl. auto.
-      intros. apply in_list_repeat in H0. subst. simpl. auto.
-Qed.
-
-Lemma encoding_shape_int : forall n i,
-  encoding_shape (encode_int n i).
-Proof.
-  unfold encode_int, inj_int. intros.
-  destruct (@bytes_of_int_prop1 (nat_of_Z (ZRdiv (Z_of_nat (S n)) 8)) 
-                                (Int.unsigned n i)) 
-    as [b [bl EQ]]; auto.
-    apply ZRdiv_prop6.
-  rewrite EQ.
-Admitted.
-
-Lemma encoding_shape_pointer : forall b i,
-  encoding_shape (inj_pointer (size_chunk_nat (Mint 31)) b i).
-Proof.
-  intros.
-  unfold size_chunk_nat, size_chunk.
-  rewrite bytesize_chunk_31_eq_4.
-  simpl.
-  apply encoding_shape_intro; simpl; auto.
-    intros.
-    unfold memval_valid_cont.
-    unfold size_chunk_nat, size_chunk. 
-    destruct H; subst; simpl; auto.
-      rewrite bytesize_chunk_31_eq_4. compute. intro. inversion H.
-    destruct H; subst; simpl; auto.
-      rewrite bytesize_chunk_31_eq_4. compute. intro. inversion H.
-    destruct H; subst; simpl; auto.
-      rewrite bytesize_chunk_31_eq_4. compute. intro. inversion H.
-      inversion H.
-Qed.
-
-Lemma encoding_shape_ipointer : forall i,
-  encoding_shape (inj_ipointer (size_chunk_nat (Mint 31)) i).
-Proof.
-  intros.
-  unfold size_chunk_nat, size_chunk.
-  rewrite bytesize_chunk_31_eq_4.
-  simpl.
-  apply encoding_shape_intro; simpl; auto.
-    intros.
-    unfold memval_valid_cont.
-    unfold size_chunk_nat, size_chunk. 
-    destruct H; subst; simpl; auto.
-      rewrite bytesize_chunk_31_eq_4. compute. intro. inversion H.
-    destruct H; subst; simpl; auto.
-      rewrite bytesize_chunk_31_eq_4. compute. intro. inversion H.
-    destruct H; subst; simpl; auto.
-      rewrite bytesize_chunk_31_eq_4. compute. intro. inversion H.
-      inversion H.
-Qed.
-
 Lemma encode_val_shape:
   forall chunk v, encoding_shape (encode_val chunk v).
 Proof.
-  intros. 
+  intros.
   destruct (size_chunk_nat_pos chunk) as [sz1 EQ].
   assert (encoding_shape (list_repeat (size_chunk_nat chunk) Undef)).
-    rewrite EQ; simpl; constructor. exact I. 
+    rewrite EQ; simpl; constructor. exact I.
     intros. replace mv with Undef. exact I. symmetry; eapply in_list_repeat; eauto.
   assert (forall bl, length bl = size_chunk_nat chunk ->
-          encoding_shape (inj_bytes bl)).
-    intros. destruct bl; simpl in *. congruence. 
+          encoding_shape (inj_bytes (wz_of_chunk chunk) bl)).
+    intros. destruct bl; simpl in *. congruence.
     constructor. exact I. unfold inj_bytes. intros.
     exploit list_in_map_inv; eauto. intros [x [A B]]. subst mv. exact I.
-  destruct v; simpl. 
-  auto.
+  destruct v; simpl.
+    auto.
+    apply H0. apply encode_int_length.
+    apply H0. apply encode_float_length.
 
-  destruct chunk; auto.
-    destruct (eq_nat_dec wz n); subst; auto.   
-      apply encoding_shape_int.
+    destruct chunk; auto.
+    destruct (eq_nat_dec n 31); auto.
+      constructor. 
+        red. auto.
+        simpl; intros. intuition; subst mv; red; simpl; congruence.
 
-  apply H0. apply encode_float_length.
-
-  destruct chunk; auto.
-    destruct (eq_nat_dec n 31); subst; auto.
-      apply encoding_shape_pointer.
-
-  destruct chunk; auto.
-    destruct (eq_nat_dec n 31); subst; auto.
-      apply encoding_shape_ipointer.
-
-(*
-  simpl; intros. intuition; subst mv; red; simpl; congruence.
-  apply H0. apply encode_int_length. 
-  apply H0. apply encode_float_length.
-  destruct chunk; auto. 
-  constructor. red. auto.
-  simpl; intros. intuition; subst mv; red; simpl; congruence.
-*)
+    destruct chunk; auto.
+    destruct (eq_nat_dec n 31); subst; simpl; auto. 
+      constructor. 
+        red. auto.
+        simpl; intros. intuition; subst mv; red; simpl; congruence.
 Qed.
 
 Lemma check_pointer_inv:
@@ -1517,168 +1216,44 @@ Inductive decoding_shape: list memval -> Prop :=
       (forall mv, In mv mvl -> memval_valid_cont mv /\ mv <> Undef) ->
       decoding_shape (mv1 :: mvl).
 
-Lemma decode_pointer_shape' : forall mvl,
-  proj_pointer mvl = Vundef \/ decoding_shape mvl.
-Proof.
-  intros.
-  unfold proj_pointer.
-  destruct mvl; auto.
-  destruct m; auto.
-  remember (check_pointer (size_chunk_nat Mint32) b i (Pointer b i n::mvl)) as R.
-  destruct R; auto.
-  right.
-  symmetry in HeqR.
-  apply check_pointer_inv in HeqR.
-  unfold size_chunk_nat, size_chunk in HeqR.
-  simpl in HeqR. 
-  rewrite bytesize_chunk_31_eq_4 in HeqR.
-  simpl in HeqR.
-  rewrite HeqR.
-  apply decoding_shape_intro; simpl; auto.
-    intro J. inversion J.
-    intros. 
-    destruct H; subst; simpl; auto.
-      split.
-        unfold size_chunk_nat, size_chunk.
-        simpl. rewrite bytesize_chunk_31_eq_4.
-        compute. intro J. inversion J.
-        intro J. inversion J.
-    destruct H; subst; simpl; auto.
-      split.
-        unfold size_chunk_nat, size_chunk.
-        simpl. rewrite bytesize_chunk_31_eq_4.
-        compute. intro J. inversion J.
-        intro J. inversion J.
-    destruct H; subst; simpl; auto.
-      split.
-        unfold size_chunk_nat, size_chunk.
-        simpl. rewrite bytesize_chunk_31_eq_4.
-        compute. intro J. inversion J.
-        intro J. inversion J.
-      inversion H.
-Qed.
-
-Lemma decode_pointer_shape'' : forall mvl,
-  proj_ipointer mvl = Vundef \/ decoding_shape mvl.
-Proof.
-  intros.
-  unfold proj_ipointer.
-  destruct mvl; auto.
-  destruct m; auto.
-  remember (check_ipointer (size_chunk_nat Mint32) i (IPointer i n::mvl)) as R.
-  destruct R; auto.
-  right.
-  symmetry in HeqR.
-  apply check_ipointer_inv in HeqR.
-  unfold size_chunk_nat, size_chunk in HeqR.
-  simpl in HeqR. 
-  rewrite bytesize_chunk_31_eq_4 in HeqR.
-  simpl in HeqR.
-  rewrite HeqR.
-  apply decoding_shape_intro; simpl; auto.
-    intro J. inversion J.
-    intros. 
-    destruct H; subst; simpl; auto.
-      split.
-        unfold size_chunk_nat, size_chunk.
-        simpl. rewrite bytesize_chunk_31_eq_4.
-        compute. intro J. inversion J.
-        intro J. inversion J.
-    destruct H; subst; simpl; auto.
-      split.
-        unfold size_chunk_nat, size_chunk.
-        simpl. rewrite bytesize_chunk_31_eq_4.
-        compute. intro J. inversion J.
-        intro J. inversion J.
-    destruct H; subst; simpl; auto.
-      split.
-        unfold size_chunk_nat, size_chunk.
-        simpl. rewrite bytesize_chunk_31_eq_4.
-        compute. intro J. inversion J.
-        intro J. inversion J.
-      inversion H.
-Qed.
-
-Lemma decoding_shape_inj_bytes : forall l,
-  (length l > 0)%nat ->
-  decoding_shape (inj_bytes l).
-Proof.
-  destruct l; intros; simpl; auto.
-    simpl in H. contradict H; omega.
-    apply decoding_shape_intro; simpl; auto.
-      intro J. inversion J.
-      intros. 
-Admitted.
-
 Lemma decode_val_shape:
   forall chunk mvl,
   List.length mvl = size_chunk_nat chunk ->
   decode_val chunk mvl = Vundef \/ decoding_shape mvl.
 Proof.
-  intros. destruct (size_chunk_nat_pos chunk) as [sz EQ]. 
+  intros. destruct (size_chunk_nat_pos chunk) as [sz EQ].
   unfold decode_val.
-  destruct chunk.
-    unfold decode_int.
-    remember (proj_int n (rev_if_be _ mvl)) as R.
-    unfold proj_int in HeqR.
-    destruct R.
-      destruct (nat_of_Z (ZRdiv (Z_of_nat (S n)) 8)).        
-        destruct (rev_if_be _ mvl); try solve [inversion HeqR].
+  caseEq (proj_bytes (wz_of_chunk chunk) mvl).
+    intros bl PROJ. right. exploit inj_proj_bytes; eauto. intros. subst mvl.
+    destruct bl; simpl in H. congruence. simpl.
+    constructor.
+      red; auto. 
+      congruence.
+      unfold inj_bytes; intros. exploit list_in_map_inv; eauto. intros [b [A B]].
+      subst mv. 
+      split. 
+        red; auto. 
+        congruence.
 
-        remember (rev_if_be _ mvl) as R'.
-        destruct R'; try solve [inversion HeqR].
-        destruct m; try solve [inversion HeqR].
-        destruct (eq_nat_dec n1 (nat_of_Z (Z_of_nat (S n) mod 8))); 
-          try solve [inversion HeqR].
-        remember (proj_bytes n0 R') as R''.
-        destruct R''; try solve [inversion HeqR].
-         right. admit.
-      destruct (eq_nat_dec n 31); subst; auto.
-        destruct (@decode_pointer_shape' mvl) as [J | J]; auto.
-          rewrite J.
-          apply decode_pointer_shape''.
+    intros. destruct chunk; auto. destruct (eq_nat_dec n 31); subst; auto.
+    unfold proj_pointer, proj_ipointer.
+    destruct mvl; auto. 
+    destruct m; auto.
+      caseEq (check_pointer (size_chunk_nat Mint32) b i (Pointer b i n :: mvl));
+        auto.
+      intros. right. exploit check_pointer_inv; eauto. simpl; intros; inv H2.
+      constructor. 
+        red. auto.  
+        congruence.
+        simpl; intros. intuition; subst mv; simpl; congruence.
 
-    unfold bytesize_chunk_nat.
-    rewrite bytesize_chunk_31_eq_4.
-    unfold size_chunk_nat, size_chunk in H. 
-    rewrite <- H.
-    remember (proj_bytes (length mvl) mvl) as R.
-    destruct R; auto.
-      symmetry in HeqR.
-      apply inj_proj_bytes in HeqR.
-      rewrite HeqR.
-      right. apply decoding_shape_inj_bytes.
-        rewrite HeqR in H.
-        rewrite length_inj_bytes in H.
-        rewrite H. compute. auto.
-         
-    unfold bytesize_chunk_nat.
-    rewrite bytesize_chunk_63_eq_8.
-    unfold size_chunk_nat, size_chunk in H. 
-    rewrite <- H.
-    remember (proj_bytes (length mvl) mvl) as R.
-    destruct R; auto.
-      symmetry in HeqR.
-      apply inj_proj_bytes in HeqR.
-      rewrite HeqR.
-      right. apply decoding_shape_inj_bytes.
-        rewrite HeqR in H.
-        rewrite length_inj_bytes in H.
-        rewrite H. compute. admit.
-(*
-  caseEq (proj_bytes mvl).
-  intros bl PROJ. right. exploit inj_proj_bytes; eauto. intros. subst mvl.
-  destruct bl; simpl in H. congruence. simpl. constructor. 
-  red; auto. congruence.
-  unfold inj_bytes; intros. exploit list_in_map_inv; eauto. intros [b [A B]]. 
-  subst mv. split. red; auto. congruence.
-  intros. destruct chunk; auto. unfold proj_pointer.
-  destruct mvl; auto. destruct m; auto. 
-  caseEq (check_pointer (size_chunk_nat Mint32) b i (Pointer b i n :: mvl)); auto.
-  intros. right. exploit check_pointer_inv; eauto. simpl; intros; inv H2.
-  constructor. red. auto. congruence. 
-  simpl; intros. intuition; subst mv; simpl; congruence.
-*)
+      caseEq (check_ipointer (size_chunk_nat Mint32) i (IPointer i n :: mvl));
+        auto.
+      intros. right. exploit check_ipointer_inv; eauto. simpl; intros; inv H2.
+      constructor. 
+        red. auto.  
+        congruence.
+        simpl; intros. intuition; subst mv; simpl; congruence.
 Qed.
 
 Lemma encode_val_pointer_inv:
@@ -1687,52 +1262,25 @@ Lemma encode_val_pointer_inv:
   chunk = Mint32 /\ v = Vptr b ofs /\ 
     mvl = inj_pointer (pred (size_chunk_nat Mint32)) b ofs.
 Proof.
-  intros until mvl. 
+  intros until mvl.
   destruct (size_chunk_nat_pos chunk) as [sz SZ].
-  unfold encode_val. rewrite SZ. destruct v.
-  simpl. congruence. 
+  unfold encode_val. rewrite SZ. 
+  destruct v.
+    simpl. congruence.
 
-  destruct chunk.
-    destruct (eq_nat_dec wz n0); subst.
-      intro.
-      unfold encode_int in H.
-      admit.
+    generalize (encode_int_length chunk wz i). 
+    destruct (encode_int chunk wz i); simpl; congruence.
 
-      intro.
-      admit.
-    intro.
-    admit.
+    generalize (encode_float_length chunk f). 
+    destruct (encode_float chunk f); simpl; congruence.
 
-    intro.
-    admit.
+    destruct chunk; try (simpl; congruence).
+    destruct (eq_nat_dec n0 31); subst; try (simpl; congruence).
+    simpl. intuition congruence.
 
-  intro. admit.
-
-
-  destruct chunk.
-    destruct (eq_nat_dec n0 31); subst.
-      intro.
-      admit.
-
-      intro.
-      admit.
-    intro.
-    admit.
-
-    intro.
-    admit.
-
-(*
-  intros until mvl. 
-  destruct (size_chunk_nat_pos chunk) as [sz SZ].
-  unfold encode_val. rewrite SZ. destruct v.
-  simpl. congruence. 
-  generalize (encode_int_length chunk i). destruct (encode_int chunk i); simpl; congruence.
-  generalize (encode_float_length chunk f). destruct (encode_float chunk f); simpl; congruence.
-  destruct chunk; try (simpl; congruence). 
-  simpl. intuition congruence. 
-*)
-Admitted.
+    destruct chunk; try (simpl; congruence).
+    destruct (eq_nat_dec n0 31); subst; try (simpl; congruence).
+Qed.
 
 Lemma encode_val_ipointer_inv:
   forall chunk v i n mvl,
@@ -1740,7 +1288,25 @@ Lemma encode_val_ipointer_inv:
   chunk = Mint32 /\ v = Vinttoptr i /\ 
     mvl = inj_ipointer (pred (size_chunk_nat Mint32)) i.
 Proof.
-Admitted.
+  intros until mvl.
+  destruct (size_chunk_nat_pos chunk) as [sz SZ].
+  unfold encode_val. rewrite SZ. 
+  destruct v.
+    simpl. congruence.
+
+    generalize (encode_int_length chunk wz i0). 
+    destruct (encode_int chunk wz i0); simpl; congruence.
+
+    generalize (encode_float_length chunk f). 
+    destruct (encode_float chunk f); simpl; congruence.
+
+    destruct chunk; try (simpl; congruence).
+    destruct (eq_nat_dec n0 31); subst; try (simpl; congruence).
+
+    destruct chunk; try (simpl; congruence).
+    destruct (eq_nat_dec n0 31); subst; try (simpl; congruence).
+    simpl. intuition congruence.
+Qed.
 
 Lemma decode_val_pointer_inv:
   forall chunk mvl b ofs,
@@ -1748,34 +1314,23 @@ Lemma decode_val_pointer_inv:
   chunk = Mint32 /\ mvl = inj_pointer (size_chunk_nat Mint32) b ofs.
 Proof.
   intros until ofs; unfold decode_val.
-  destruct chunk.
-    unfold decode_int.
-    destruct (proj_int n (rev_if_be _ mvl)).
-      intro J. inversion J.
-      destruct (eq_nat_dec n 31); subst.
-        intro J. split; auto.
-          admit.          
+  destruct (proj_bytes (wz_of_chunk chunk) mvl).
+    destruct chunk; congruence.
 
-        intro J. inversion J.
-
-    destruct (proj_bytes (bytesize_chunk_nat 31) mvl).
-      intro J. inversion J.
-      intro J. inversion J.
-
-    destruct (proj_bytes (bytesize_chunk_nat 63) mvl).
-      intro J. inversion J.
-      intro J. inversion J.
-
-(*
-  intros until ofs; unfold decode_val.
-  destruct (proj_bytes mvl). 
-  destruct chunk; congruence.
-  destruct chunk; try congruence.
-  unfold proj_pointer. destruct mvl. congruence. destruct m; try congruence.
-  case_eq (check_pointer (size_chunk_nat Mint32) b0 i (Pointer b0 i n :: mvl)); intros.
-  inv H0. split; auto. apply check_pointer_inv; auto. 
-  congruence.
-*)
+    destruct chunk; try congruence.
+    destruct (eq_nat_dec n 31); subst; try congruence.
+    unfold proj_pointer. 
+    Opaque check_ipointer.
+    destruct mvl; try solve [intro J; inversion J].
+    destruct m; try solve [intro J; inversion J].
+      case_eq (check_pointer (size_chunk_nat Mint32) b0 i 
+        (Pointer b0 i n :: mvl)); intros.
+        inv H0. split; auto. apply check_pointer_inv; auto.
+        inv H0.
+      intro J. simpl in J.
+      destruct (check_ipointer (size_chunk_nat Mint32) i (IPointer i n :: mvl));
+        inversion J.
+    Transparent check_ipointer.
 Qed.
 
 Lemma decode_val_ipointer_inv:
@@ -1784,23 +1339,25 @@ Lemma decode_val_ipointer_inv:
   chunk = Mint32 /\ mvl = inj_ipointer (size_chunk_nat Mint32) i.
 Proof.
   intros until i; unfold decode_val.
-  destruct chunk.
-    unfold decode_int.
-    destruct (proj_int n (rev_if_be _ mvl)).
-      intro J. inversion J.
-      destruct (eq_nat_dec n 31); subst.
-        intro J. split; auto.
-          admit.          
+  destruct (proj_bytes (wz_of_chunk chunk) mvl).
+    destruct chunk; congruence.
 
-        intro J. inversion J.
+    destruct chunk; try congruence.
+    destruct (eq_nat_dec n 31); subst; try congruence.
+    unfold proj_ipointer. 
+    unfold proj_pointer.
+    Opaque check_pointer.
+    destruct mvl; try congruence.
+    destruct m; try congruence.
+      case_eq (check_pointer (size_chunk_nat Mint32) b i0 
+        (Pointer b i0 n :: mvl)); intros.
+        inv H0. inv H0.
 
-    destruct (proj_bytes (bytesize_chunk_nat 31) mvl).
-      intro J. inversion J.
-      intro J. inversion J.
-
-    destruct (proj_bytes (bytesize_chunk_nat 63) mvl).
-      intro J. inversion J.
-      intro J. inversion J.
+      case_eq (check_ipointer (size_chunk_nat Mint32) i0 (IPointer i0 n :: mvl));
+        intros.
+        inv H0. split; auto. apply check_ipointer_inv; auto.
+        inv H0.
+    Transparent check_pointer.
 Qed.
 
 Inductive pointer_encoding_shape: list memval -> Prop :=
@@ -1813,56 +1370,18 @@ Lemma encode_pointer_shape:
   forall b ofs, pointer_encoding_shape (encode_val Mint32 (Vptr b ofs)).
 Proof.
   intros. simpl. 
-  unfold size_chunk_nat, size_chunk.
-  rewrite bytesize_chunk_31_eq_4. simpl.
   constructor.
-  unfold memval_valid_cont. red; intro. elim H. auto. 
-  unfold memval_valid_first. simpl; intros; intuition; subst mv.
-    unfold size_chunk_nat, size_chunk in H0.
-    simpl in H0. rewrite bytesize_chunk_31_eq_4 in H0. 
-    contradict H0. compute. intro J. inversion J.
-    
-    unfold size_chunk_nat, size_chunk in H0.
-    simpl in H0. rewrite bytesize_chunk_31_eq_4 in H0. 
-    contradict H0. compute. intro J. inversion J.
-
-    unfold size_chunk_nat, size_chunk in H0.
-    simpl in H0. rewrite bytesize_chunk_31_eq_4 in H0. 
-    contradict H0. compute. intro J. inversion J.
-
-(*
-  intros. simpl. constructor.
-  unfold memval_valid_cont. red; intro. elim H. auto. 
-  unfold memval_valid_first. simpl; intros; intuition; subst mv; congruence.
-*)
+    unfold memval_valid_cont. red; intro. elim H. auto.
+    unfold memval_valid_first. simpl; intros; intuition; subst mv; congruence.
 Qed.
 
 Lemma encode_ipointer_shape:
   forall i, pointer_encoding_shape (encode_val Mint32 (Vinttoptr i)).
 Proof.
   intros. simpl. 
-  unfold size_chunk_nat, size_chunk.
-  rewrite bytesize_chunk_31_eq_4. simpl.
   constructor.
-  unfold memval_valid_cont. red; intro. elim H. auto. 
-  unfold memval_valid_first. simpl; intros; intuition; subst mv.
-    unfold size_chunk_nat, size_chunk in H0.
-    simpl in H0. rewrite bytesize_chunk_31_eq_4 in H0. 
-    contradict H0. compute. intro J. inversion J.
-    
-    unfold size_chunk_nat, size_chunk in H0.
-    simpl in H0. rewrite bytesize_chunk_31_eq_4 in H0. 
-    contradict H0. compute. intro J. inversion J.
-
-    unfold size_chunk_nat, size_chunk in H0.
-    simpl in H0. rewrite bytesize_chunk_31_eq_4 in H0. 
-    contradict H0. compute. intro J. inversion J.
-
-(*
-  intros. simpl. constructor.
-  unfold memval_valid_cont. red; intro. elim H. auto. 
-  unfold memval_valid_first. simpl; intros; intuition; subst mv; congruence.
-*)
+    unfold memval_valid_cont. red; intro. elim H. auto.
+    unfold memval_valid_first. simpl; intros; intuition; subst mv; congruence.
 Qed.
 
 Lemma decode_pointer_shape:
@@ -1871,8 +1390,7 @@ Lemma decode_pointer_shape:
   chunk = Mint32 /\ pointer_encoding_shape mvl.
 Proof.
   intros. exploit decode_val_pointer_inv; eauto. intros [A B].
-  split; auto. subst mvl.
-
+  split; auto. subst mvl. 
   assert (J:=@encode_pointer_shape b ofs).
   unfold encode_val in J.
   simpl in J. auto.
@@ -1885,7 +1403,6 @@ Lemma decode_ipointer_shape:
 Proof.
   intros. exploit decode_val_ipointer_inv; eauto. intros [A B].
   split; auto. subst mvl.
-
   assert (J:=@encode_ipointer_shape i).
   unfold encode_val in J.
   simpl in J. auto.
@@ -1928,52 +1445,12 @@ Proof.
   inv H; try congruence.
 
   intros.
-  destruct n0; simpl in *; auto.
-    destruct (eq_nat_dec wz 8); auto.
-      remember (proj_bytes n0 al) as R.
-      destruct R.
-        rewrite (IHlist_forall2 n0 l); auto.
-        inversion H.
-
-  intros.
-  destruct n0; simpl in *; auto.
-
-  intros.
-  destruct n0; simpl in *; auto.
-
-  intros.
-  destruct n; simpl in *; auto.
-    inversion H.
+  destruct (eq_nat_dec wz n0); auto.
+  remember (proj_bytes n0 al) as R.
+  destruct R.
+    inv H. rewrite (IHlist_forall2 n0 l); auto.
+    congruence.      
 Qed.
-
-Lemma proj_int_inject:
-  forall f vl vl',
-  list_forall2 (memval_inject f) vl vl' ->
-  forall n i,
-  proj_int n vl = Some i ->
-  proj_int n vl' = Some i.
-Proof.
-  intros.
-  unfold proj_int in *.
-  destruct (nat_of_Z (ZRdiv (Z_of_nat (S n)) 8)); auto.
-    destruct vl; destruct vl'; auto.
-
-  destruct vl; destruct vl'; auto.
-    inversion H0.
-    inversion H.
-
-  destruct m; destruct m0; auto; try solve 
-    [inversion H0 | inversion H; subst; inversion H4].
-
-    inversion H; subst. inversion H4; subst.
-    destruct (eq_nat_dec n2 (nat_of_Z (Z_of_nat (S n) mod 8))); auto.
-    remember (proj_bytes n0 vl) as R.
-    destruct R.
-      apply proj_bytes_inject with (n:=n0)(bl:=l) in H6; auto.
-      rewrite H6. auto.
-
-      inversion H0.
-Qed.  
 
 Lemma check_pointer_inject:
   forall f vl vl',
@@ -1983,16 +1460,16 @@ Lemma check_pointer_inject:
   f b = Some(b', delta) ->
   check_pointer n b' (Int.add 31 ofs (Int.repr 31 delta)) vl' = true.
 Proof.
-  induction 1; intros; destruct n; simpl in *; auto. 
+  induction 1; intros; destruct n; simpl in *; auto.
   inv H; auto.
-  destruct (andb_prop _ _ H1). destruct (andb_prop _ _ H). 
-  destruct (andb_prop _ _ H5). 
+  destruct (andb_prop _ _ H1). destruct (andb_prop _ _ H).
+  destruct (andb_prop _ _ H5).
   assert (n = n0) by (apply beq_nat_true; auto).
-  assert (b = b0) by (eapply proj_sumbool_true; eauto). 
+  assert (b = b0) by (eapply proj_sumbool_true; eauto).
   assert (ofs = ofs1) by (eapply proj_sumbool_true; eauto).
-  subst. rewrite H3 in H2; inv H2. 
-  unfold proj_sumbool. rewrite dec_eq_true. rewrite dec_eq_true. 
-  rewrite <- beq_nat_refl. simpl. eauto. 
+  subst. rewrite H3 in H2; inv H2.
+  unfold proj_sumbool. rewrite dec_eq_true. rewrite dec_eq_true.
+  rewrite <- beq_nat_refl. simpl. eauto.
   congruence.
 Qed.
 
@@ -2048,67 +1525,17 @@ Lemma proj_bytes_not_inject:
   proj_bytes n vl = None -> proj_bytes n vl' <> None -> In Undef vl.
 Proof.
   induction 1; simpl; intros.
-  congruence.
-  inv H; try congruence. 
-
-  destruct n; simpl in H1, H2; auto.
-    contradict H2; auto.
-    destruct (eq_nat_dec wz 8); subst.
+    congruence.
+    inv H; try congruence; auto.
+    destruct (eq_nat_dec wz n); subst; auto.
       remember (proj_bytes n al) as R.
       remember (proj_bytes n bl) as R'.
       destruct R; destruct R';
         try solve [inversion H1 | inversion H2 | contradict H2; auto].
         right. eapply IHlist_forall2; eauto.
           rewrite <- HeqR'. intro. inversion H.          
-    contradict H2; auto.
-
-  destruct n; simpl in H2; contradict H2; auto.     
-
-  destruct n; simpl in H2; contradict H2; auto.     
-  
-  auto.
-
-(*
-  induction 1; simpl; intros.
-  congruence.
-  inv H; try congruence. 
-  right. apply IHlist_forall2.
-  destruct (proj_bytes al); congruence.
-  destruct (proj_bytes bl); congruence.
-  auto.
-*)
+      contradict H2; auto.
 Qed.
-
-Lemma proj_int_not_inject:
-  forall f vl vl',
-  list_forall2 (memval_inject f) vl vl' ->
-  forall n,
-  proj_int n vl = None ->
-  proj_int n vl' <> None ->
-  In Undef vl.
-Proof.
-  intros.
-  unfold proj_int in *.
-  destruct (nat_of_Z (ZRdiv (Z_of_nat (S n)) 8)); auto.
-    destruct vl'; contradict H1; auto.
-
-  destruct vl; destruct vl'; auto.
-    contradict H1; auto.
-    inversion H.
-    contradict H1; auto.
-
-  destruct m; destruct m0; auto; try solve 
-    [simpl; auto | contradict H1; auto | inversion H; subst; inversion H5].
-
-    inversion H; subst. inversion H5; subst.
-    remember (proj_bytes n0 vl) as R.
-    remember (proj_bytes n0 vl') as R'.
-    destruct (eq_nat_dec n2 (nat_of_Z (Z_of_nat (S n) mod 8)));
-      try solve [contradict H1; auto].
-      destruct R; destruct R'; try solve [inversion H0 | contradict H1; auto].
-        apply proj_bytes_not_inject with (n:=n0) in H7; simpl; auto.
-          rewrite <- HeqR'. intro J. inversion J.
-Qed.  
 
 Lemma check_pointer_undef:
   forall n b ofs vl,
@@ -2148,22 +1575,51 @@ Proof.
   rewrite check_ipointer_undef. auto. auto.
 Qed.
 
-Lemma list_forall2_memval_inject_rev_if_be : forall f vl1 vl2,
-  list_forall2 (memval_inject f) vl1 vl2 ->
-  list_forall2 (memval_inject f) (rev_if_be _ vl1) (rev_if_be _ vl2).
+Lemma proj_bytes_undef:
+  forall vl wz, In Undef vl -> proj_bytes wz vl = None.
 Proof.
-  induction vl1; intros.
-    inversion H; subst.
-    unfold rev_if_be.
-    destruct big_endian; simpl; auto.
-  
-    inversion H; subst.
-    apply IHvl1 in H4.
-    unfold rev_if_be in *.
-    destruct big_endian; simpl; auto.
-      apply list_forall2_app; auto.
-        apply list_forall2_cons; auto.
-          apply list_forall2_nil.
+  induction vl; intros. 
+    inversion H.   
+
+    simpl in H.
+    destruct H as [H | H]; simpl; subst; auto.
+    destruct a; auto.
+    destruct (eq_nat_dec n wz); subst; auto.
+    rewrite IHvl; auto.
+Qed.
+
+Lemma proj_pointer_inv : forall vs,
+  proj_pointer vs = Vundef \/ exists b, exists ofs, proj_pointer vs = Vptr b ofs.
+Proof.
+  intros.
+  unfold proj_pointer.
+  destruct vs; auto.
+  destruct m; auto.
+  destruct (check_pointer (size_chunk_nat Mint32) b i (Pointer b i n :: vs));
+    auto.
+    right. exists b. exists i. auto.
+Qed.
+
+Lemma proj_ipointer_inv : forall vs,
+  proj_ipointer vs = Vundef \/ exists i, proj_ipointer vs = Vinttoptr i.
+Proof.
+  intros.
+  unfold proj_ipointer.
+  destruct vs; auto.
+  destruct m; auto.
+  destruct (check_ipointer (size_chunk_nat Mint32) i (IPointer i n :: vs)); auto.
+    right. exists i. auto.
+Qed.
+
+Lemma proj_pointer_neq_proj_ipointer : forall vs,
+  proj_pointer vs <> Vundef ->
+  proj_ipointer vs <> Vundef ->
+  False.
+Proof.
+  unfold proj_pointer, proj_ipointer. intros.
+  destruct vs; try solve [contradict H; auto].
+  destruct m; try solve [contradict H; auto].
+    auto.
 Qed.
 
 Theorem decode_val_inject:
@@ -2171,63 +1627,36 @@ Theorem decode_val_inject:
   list_forall2 (memval_inject f) vl1 vl2 ->
   val_inject f (decode_val chunk vl1) (decode_val chunk vl2).
 Proof.
-  intros. unfold decode_val. 
-  destruct chunk.
-    unfold decode_int.
-    apply list_forall2_memval_inject_rev_if_be in H.
-    remember (proj_int n (rev_if_be memval vl1)) as R.
-    remember (proj_int n (rev_if_be memval vl2)) as R'.
-    destruct R; destruct R'; auto.
-      rewrite proj_int_inject with (f:=f)(vl:=rev_if_be _ vl1)
-        (vl':=rev_if_be _ vl2) (i:=i) in HeqR'; auto.
-        inversion HeqR'; auto.
-      rewrite proj_int_inject with (f:=f)(vl:=rev_if_be _ vl1)
-        (vl':=rev_if_be _ vl2) (i:=i) in HeqR'; auto.
-        inversion HeqR'; auto.
+  intros. unfold decode_val.
+  case_eq (proj_bytes (wz_of_chunk chunk) vl1); intros.
+    exploit proj_bytes_inject; eauto. intros. rewrite H1.
+    destruct chunk; constructor.
+ 
+    destruct chunk; auto.
+    destruct (eq_nat_dec n 31); subst; auto.
+    case_eq (proj_bytes (wz_of_chunk (Mint 31)) vl2); intros.
+      assert (In Undef vl1) as J.
+        eapply proj_bytes_not_inject; eauto. 
+           congruence.
+      rewrite proj_pointer_undef; auto.
+      rewrite proj_ipointer_undef; auto.
+      destruct (@proj_pointer_inv vl1) as [J1 | [b1 [ofs1 J1]]]; rewrite J1.
+        destruct (@proj_ipointer_inv vl1) as [J1' | [i1' J1']]; rewrite J1'. 
+          auto.
+        apply proj_ipointer_inject in H.
+        rewrite J1' in H.
+        destruct (@proj_pointer_inv vl2) as [J2 | [b2 [ofs2 J2]]]; rewrite J2.
+          auto.
 
-      symmetry in HeqR.
-      apply proj_int_not_inject with (n:=n) in H; auto.
-        destruct (eq_nat_dec n 31); subst; auto.
-        rewrite proj_pointer_undef; auto.
-          rewrite proj_ipointer_undef; auto.
-          admit.
-        admit.
+          inv H.
+          case_eq (proj_pointer_neq_proj_ipointer vl2); try congruence.
 
-        rewrite <- HeqR'. intro J. inversion J.
-
-      destruct (eq_nat_dec n 31); subst; auto.
-        unfold proj_pointer.
-        admit.
-
-    remember (proj_bytes (bytesize_chunk_nat 31) vl1) as R.
-    remember (proj_bytes (bytesize_chunk_nat 31) vl2) as R'.
-    destruct R; destruct R'; auto.
-      rewrite proj_bytes_inject with (f:=f)(vl:=vl1)(vl':=vl2)(bl:=l) in HeqR'; 
-        auto.
-        inversion HeqR'; auto.
-      rewrite proj_bytes_inject with (f:=f)(vl:=vl1)(vl':=vl2)(bl:=l) in HeqR'; 
-        auto.
-        inversion HeqR'; auto.
-
-    remember (proj_bytes (bytesize_chunk_nat 63) vl1) as R.
-    remember (proj_bytes (bytesize_chunk_nat 63) vl2) as R'.
-    destruct R; destruct R'; auto.
-      rewrite proj_bytes_inject with (f:=f)(vl:=vl1)(vl':=vl2)(bl:=l) in HeqR';
-        auto.
-        inversion HeqR'; auto.
-      rewrite proj_bytes_inject with (f:=f)(vl:=vl1)(vl':=vl2)(bl:=l) in HeqR'; 
-        auto.
-        inversion HeqR'; auto.
-
-(*
-  case_eq (proj_bytes vl1); intros. 
-  exploit proj_bytes_inject; eauto. intros. rewrite H1. 
-  destruct chunk; constructor.
-  destruct chunk; auto.
-  case_eq (proj_bytes vl2); intros.
-  rewrite proj_pointer_undef. auto. eapply proj_bytes_not_inject; eauto. congruence.
-  apply proj_pointer_inject; auto.
-*)
+        destruct (@proj_pointer_inv vl2) as [J2 | [b2 [ofs2 J2]]]; rewrite J2.
+          apply proj_pointer_inject in H.
+          rewrite J1 in H. rewrite J2 in H. inversion H.
+           
+          rewrite <- J1. rewrite <- J2.
+          apply proj_pointer_inject; auto.
 Qed.
 
 (** Symmetrically, [encode_val], applied to values related by [val_inject],
@@ -2235,21 +1664,10 @@ Qed.
   related by [memval_inject]. *)
 
 Lemma inj_bytes_inject:
-  forall f bl, list_forall2 (memval_inject f) (inj_bytes bl) (inj_bytes bl).
+  forall f wz bl, 
+    list_forall2 (memval_inject f) (inj_bytes wz bl) (inj_bytes wz bl).
 Proof.
   induction bl; constructor; auto. constructor.
-Qed.
-
-Lemma inj_int_inject:
-  forall f n i, list_forall2 (memval_inject f) (inj_int n i) (inj_int n i).
-Proof.
-  intros.
-  unfold inj_int.
-  destruct (bytes_of_int (nat_of_Z (ZRdiv (Z_of_nat (S n)) 8)) (Int.unsigned n i)).
-    apply list_forall2_nil.
-    apply list_forall2_cons.
-      apply memval_inject_byte.
-      apply inj_bytes_inject.
 Qed.
 
 Lemma repeat_Undef_inject_any:
@@ -2272,51 +1690,19 @@ Theorem encode_val_inject:
   list_forall2 (memval_inject f) (encode_val chunk v1) (encode_val chunk v2).
 Proof.
   intros. inv H; simpl.
+    apply inj_bytes_inject.
+    apply inj_bytes_inject.
 
-  destruct chunk.
-    destruct (eq_nat_dec wz n); subst.
-      unfold encode_int.
-      apply list_forall2_memval_inject_rev_if_be.
-      apply inj_int_inject.
+    destruct chunk; try apply repeat_Undef_inject_self.
+    destruct (eq_nat_dec n 31); subst; try apply repeat_Undef_inject_self.
+      simpl; repeat econstructor; auto.
 
-      apply repeat_Undef_inject_self.
-   apply repeat_Undef_inject_self.
-   apply repeat_Undef_inject_self.
-   apply inj_bytes_inject.
-
-
-  destruct chunk.
-    destruct (eq_nat_dec n 31); subst.
-      unfold size_chunk_nat, size_chunk.     
-      rewrite bytesize_chunk_31_eq_4.
-      unfold inj_pointer; simpl; repeat econstructor; auto.
-
-      apply repeat_Undef_inject_self.
-   apply repeat_Undef_inject_self.
-   apply repeat_Undef_inject_self.
-
-  destruct chunk.
-    destruct (eq_nat_dec n 31); subst.
-      unfold size_chunk_nat, size_chunk.     
-      rewrite bytesize_chunk_31_eq_4.
+    destruct chunk; try apply repeat_Undef_inject_self.
+    destruct (eq_nat_dec n 31); subst; try apply repeat_Undef_inject_self.
       unfold inj_ipointer; simpl; repeat econstructor; auto.
 
-      apply repeat_Undef_inject_self.
-   apply repeat_Undef_inject_self.
-   apply repeat_Undef_inject_self.
-
-  rewrite <- encode_val_length with (v:=v2).
-  apply repeat_Undef_inject_any.
-
-(*
-  intros. inv H; simpl.
-  apply inj_bytes_inject.
-  apply inj_bytes_inject.
-  destruct chunk; try apply repeat_Undef_inject_self. 
-  unfold inj_pointer; simpl; repeat econstructor; auto. 
-  replace (size_chunk_nat chunk) with (length (encode_val chunk v2)).
-  apply repeat_Undef_inject_any. apply encode_val_length. 
-*)
+    replace (size_chunk_nat chunk) with (length (encode_val chunk v2)).
+    apply repeat_Undef_inject_any. apply encode_val_length.
 Qed.
 
 (** The identity injection has interesting properties. *)
